

# Sequences, Series, and Multivariable Calculus (MATH 408D) – Techniques of Integration

Dawson Zhang | Instructor: Dr. Sarower

Fall 2025

## 0.1 u-Substitution Review

u-Substitution is one of the most useful and prioritized tools when it comes to solving antiderivatives. The antiderivative power-rule doesn't help us evaluate integrals such as

$$\int 2x\sqrt{1+x^2}dx$$

**Remark 0.1.** To find this integral, we can change the variable  $x$  into another variable to simplify the integration process.

*Solution.* Consider setting  $1+x^2$  to another variable  $u$

$$u = 1 + x^2$$

Taking the derivative of  $u$  with respect to  $x$  yields

$$\begin{aligned}u' &= \frac{du}{dx} = 2x \\ \frac{du}{2x} &= dx\end{aligned}$$

Substituting  $u$  and  $dx$  back into the original equation,

$$\int \frac{2x\sqrt{u}}{2x}du = \int \sqrt{u}du = \frac{2}{3}u^{3/2} + C$$

Finally, plugging in the original  $u$ ,

$$= \boxed{\frac{2}{3}(1+x^2)^{3/2} + C}$$

□

**Remark 0.2.** For the most part, u-substitution usually involves setting the “inside” function to  $u$ .

### Theorem 0.3

If  $u = g(x)$  is a differentiable function whose range is an interval  $I$  and  $f$  is continuous on  $I$ , then

$$\int f(g(x))g'(x)dx = \int f(u)du$$

**Example 0.4**

$$\int \cos(5x) dx$$

*Solution.* Set up u-substitution terms

$$\begin{aligned} u &= 5x \\ \frac{du}{dx} &= 5 \\ \frac{du}{5} &= dx \end{aligned}$$

Substitute into original equation

$$\begin{aligned} \int \cos(5x) dx &= \frac{1}{5} \int \cos(u) du \\ &= \frac{1}{5} \sin(u) + C \\ &= \boxed{\frac{1}{5} \sin(5x) + C} \end{aligned}$$

□

**Example 0.5**

$$\int_0^2 2x(x^2 + 1)^3 dx$$

*Solution.* Set up u-substitution terms

$$\begin{aligned} u &= x^2 + 1 \\ \frac{du}{dx} &= 2x \\ \frac{du}{2x} &= dx \end{aligned}$$

Substitute into original equation

$$\begin{aligned} \int_0^2 2x(x^2 + 1)^3 dx &= \int_0^2 \frac{2x(u)^3}{2x} du \\ &= \int_0^2 u^3 du \\ &= \frac{1}{4} u^4 \Big|_0^2 \\ &= \frac{1}{4} (x^2 + 1)^4 \Big|_0^2 \end{aligned}$$

$$= \boxed{156}$$

**Remark 0.6.** In this solution, I chose to substitute the  $u = x^2 + 1$  equation back into my solved integral instead of finding new limits of integration with respect to  $u$ .

□

### Example 0.7

$$\int_0^1 \frac{x}{1+x^2} dx$$

*Solution.*

$$\begin{aligned} u &= 1 + x^2 \\ \frac{du}{dx} &= 2x \\ dx &= \frac{du}{2x} \end{aligned}$$

□

$$\begin{aligned} \int_0^1 \frac{x}{1+x^2} dx &= \int_0^1 \frac{x}{u(2x)} du \\ &= \frac{1}{2} \int_0^2 \frac{1}{u} du \\ &= \frac{1}{2} \ln(|u|) \Big|_1^2 \\ &= \boxed{\frac{1}{2} \ln(2)} \end{aligned}$$

# 1 Integration by Parts

Integration by parts comes from the product rule from derivatives. Consider the product rule where  $f = f(x)$  and  $g = g(x)$

$$(fg)' = f'g + fg'$$

Integrate both sides of the equation

$$\int (fg)' dx = \int f'g dx + \int fg' dx$$

$$fg = \int f'g dx + \int fg' dx$$

$$\int fg' dx = fg - \int f'g dx$$

## Theorem 1.1

If  $f$  and  $g$  are differentiable functions then,

$$\int f(x)g'(x)dx = f(x)g(x) - \int g(x)f'(x)dx$$

or, equivalently,

$$\int u dv = uv - \int v du$$

where  $u = f(x)$  and  $v = g(x)$

## 1.1 Steps to consider

- Look for a product of two functions, e.g.  $f(x)g(x)$
- Choose  $u$  and  $dv$
- Choose  $u$  in order of **L.I.A.T.E** (logarithmic, inverse trig, algebraic, trig, exponential), choose  $u$  in that order

**Remark 1.2.** In practice, once integration by parts becomes more fluid, it's not necessary to consider the **L.I.A.T.E** rule every time.

- Differentiate  $u$  to find  $du$
- Integrate  $dv$  to find  $v$
- Plug into formula  $\int u dv = uv - \int v du$  and solve

**Example 1.3**

$$\int x e^x dx$$

*Solution.* Find  $u$  and  $dv$

$$\begin{aligned}u &= x \\ dv &= e^x dx\end{aligned}$$

Find  $du$

$$\begin{aligned}u &= x \\ \frac{du}{dx} &= 1 \\ du &= dx\end{aligned}$$

Find  $v$

$$\begin{aligned}dv &= e^x dx \\ \int dv &= \int e^x dx \\ v &= e^x\end{aligned}$$

Plug back into equation  $\int u dv = uv - \int v du$

$$\begin{aligned}\int x e^x dx &= x e^x - \int e^x dx \\ &= \boxed{x e^x - e^x + C}\end{aligned}$$

□

**Example 1.4**

$$\int \ln(x) dx$$

*Solution.*

$$\begin{aligned}u &= \ln(x) \\ \frac{du}{dx} &= \frac{1}{x} \\ du &= \frac{1}{x} dx\end{aligned}$$

$$dv = dx$$

$$\int dv = \int dx$$

$$v = x$$

Plug back into equation  $\int u dv = uv - \int v du$

$$\begin{aligned}\int \ln(x) dx &= x \ln(x) - \int \frac{x}{x} dx \\ &= \boxed{x \ln(x) - x + C}\end{aligned}$$

□

### Example 1.5

$$\int x \sin(x) dx$$

*Solution.*

$$\begin{aligned}u &= x \\ \frac{du}{dx} &= 1 \\ du &= dx\end{aligned}$$

$$\begin{aligned}dv &= \sin(x) dx \\ \int dv &= \int \sin(x) dx \\ v &= -\cos(x)\end{aligned}$$

Plug back into equation  $\int u dv = uv - \int v du$

$$\begin{aligned}\int x \sin(x) &= -x \cos(x) + \int \cos(x) dx \\ &= \boxed{-x \cos(x) + \sin(x)}\end{aligned}$$

□

### Example 1.6

$$\int e^x \cos(x) dx$$

*Solution.*

$$u = \cos(x)$$

$$du = -\sin(x)dx$$

$$dv = e^x dx$$

$$v = e^x$$

$$\int e^x \cos(x) dx = e^x \cos(x) + \int e^x \sin(x) dx$$

$$u = \sin(x)$$

$$du = \cos(x)dx$$

$$dv = e^x dx$$

$$v = e^x$$

$$\int e^x \cos(x) dx = e^x \cos(x) + \int e^x \sin(x) dx$$

$$= e^x \cos(x) + e^x \sin(x) - \int e^x \cos(x) dx$$

$$2 \int e^x \cos(x) dx = e^x \cos(x) + e^x \sin(x)$$

$$\int e^x \cos(x) dx = \boxed{\frac{e^x \cos(x) + e^x \sin(x)}{2} + C}$$

□

**Example 1.7**

$$\int_0^1 \arctan(x) dx$$

## 2 Trigonometric Integration

### 2.1 Review of Trig Identities

$$\sin^2(x) + \cos^2(x) = 1 \tag{1}$$

$$\sec^2(x) - \tan^2(x) = 1 \tag{2}$$

$$\csc^2(x) - \cot^2(x) = 1 \tag{3}$$

$$\tag{4}$$

$$\sin(2x) = 2 \sin(x) \cos(x) \tag{5}$$



$$\cos(2x) = \cos^2(x) - \sin^2(x) \quad (6)$$

$$\sin^2 x = \frac{1 - \cos(2x)}{2} \quad (7)$$

$$\cos^2 x = \frac{1 + \cos(2x)}{2} \quad (8)$$

$$(9)$$

### Example 2.1

$$\int \cos^5(x) dx$$

*Solution.* Plug in pythagorean identities:

$$\begin{aligned} \int \cos^5(x) dx &= \int \cos^4(x) \cos(x) dx \\ &= \int (1 - \sin^2(x))^2 \cos(x) dx \end{aligned}$$

Use u-substitution:

$$\begin{aligned} u &= \sin(x) \\ \frac{du}{dx} &= \cos(x) \\ du &= \cos(x) dx \end{aligned}$$

Solve:

$$\int \cos^5(x) dx = \int (1 - u^2)^2 du$$

**Remark 2.2.** Clever students have noticed that  $u = 1 - \sin^2(x)$  is probably easier

□

## 2.2 Products of sine and cosine

### Example 2.3

$$\int \sin^5(x) \cos^2(x) dx$$

*Solution.* Plug in pythagorean identities:

$$\begin{aligned}\int \sin^5(x) \cos^2(x) dx &= \int \sin^4(x) \cos^2(x) \sin(x) dx \\ &= \int (1 - \cos^2(x))^2 \cos^2(x) \sin(x) dx\end{aligned}$$

Use u-substitution:

$$\begin{aligned}u &= \cos(x) \\ \frac{du}{dx} &= -\sin(x) \\ du &= -\sin(x) dx\end{aligned}$$

Solve:

$$\int \sin^5(x) \cos^2(x) dx = - \int (1 - u^2)^2 u^2 du$$

□

#### Example 2.4

$$\int \sin^2(x) \cos^2(x) dx$$

*Solution.* Plug in identities

$$\begin{aligned}\int \sin^2(x) \cos^2(x) dx &= \int \frac{1 - \cos(2x)}{2} \times \frac{1 + \cos(2x)}{2} dx \\ &= \frac{1}{4} \int 1 - \cos^2(2x) dx \\ &= \frac{1}{4} \int \sin^2(2x) dx \\ &= \frac{1}{4} \int \frac{1 - \cos(4x)}{2} dx \\ &= \frac{1}{8} \int 1 - \cos(4x) dx\end{aligned}$$

□

## 2.3 Products of secant and tangent

#### Example 2.5

$$\int \sec^4 x dx$$

*Solution.*

$$\begin{aligned}
 \int \sec^4 x dx &= \int \sec^2 x \sec^2 x dx \\
 u &= \tan x \\
 du &= \sec^2 x dx \\
 &= \int (1 + \tan^2 x) \sec^2 x dx \\
 &= \int (1 + u^2) du
 \end{aligned}$$

□

### Example 2.6

$$\int \tan^6 x \sec^4 x dx$$

*Solution.*

$$\begin{aligned}
 \int \tan^6 x \sec^4 x dx &= \int \tan^6 x \sec^2 x \sec^2 x dx \\
 &= \int \tan^6 x (1 + \tan^2 x) \sec^2 x dx \\
 u &= \tan x \\
 du &= \sec^2 x dx \\
 &= \int u^6 (1 + u^2) du
 \end{aligned}$$

□

### Example 2.7

$$\int \tan^5 x \sec^7 x dx$$

*Solution.*

$$\begin{aligned}
 \int \tan^5 x \sec^7 x dx &= \int \tan^4 x \sec^6 x \tan x \sec x dx \\
 &= \int (\sec^2 x - 1)^2 \sec^6 x \tan x \sec x dx \\
 u &= \sec x \\
 du &= \tan x \sec x dx \\
 &= \int (u^2 - 1)^2 u^6 du
 \end{aligned}$$

□

**Example 2.8**

$$\int \sec^2 x \tan^3 x dx$$

*Solution.*

$$\begin{aligned} u &= \tan x \\ du &= \sec^2 x dx \\ \int \sec^2 x \tan^3 x dx &= u^3 du \\ &= \frac{1}{4} u^4 + C \\ &= \boxed{\frac{1}{4} \tan^4 x + C} \end{aligned}$$

□

**2.4 Product of sine and cosine with different angles**

$$\begin{aligned} \sin A \cos B &= \frac{1}{2}(\sin(A+B) + \sin(A-B)) \\ \sin A \sin B &= \frac{1}{2}(\cos(A-B) - \cos(A+B)) \\ \cos A \cos B &= \frac{1}{2}(\cos(A-B) + \cos(A+B)) \end{aligned}$$

**Example 2.9**

$$\int \sin(3x) \cos(2x) dx$$

*Solution.*

$$\int \sin(3x) \cos(2x) dx = \frac{1}{2} \int (\sin(5x) + \sin x) dx$$

□